Soundness.v
@@ -5,7 +5,6 @@ Require Import Classes.Joinable.
 Require Import Classes.Monad.
 Require Import Classes.Monad.MonadFail.
 Require Import Classes.PreorderedSet.
-Require Import Classes.SoundMonad.
 Require Import Coq.Arith.Arith.
 Require Import Coq.Arith.Even.
 Require Import Coq.Arith.PeanoNat.
@@ -43,127 +42,105 @@ Qed.
 Hint Extern 3 (γ (?f ?x) (?g ?y)) => apply gamma_fun_apply : soundness.
 
 (* Soundness of monadic operations *)
-Lemma some_sound {A A' : Type} `{Galois A A'} : ∀ a a', 
-  γ a a' →
-  γ (Some a) (Some a').
+Instance some_sound : return_sound option option.
 Proof.
+  unfold return_sound. eauto with soundness.
+Qed.
+
+Instance bind_option_sound : bind_sound option option.
+Proof.
+  unfold bind_sound. unfold bindM; simpl. intros. destruct m, m'; 
   eauto with soundness.
 Qed.
 
-Lemma bind_option_sound {A A' B B'} `{Galois A A', Galois B B'} : 
-  ∀ m m' f f', 
-  γ m m' → γ f f' →
-  γ (bind_option m f) (bind_option m' f').
+Instance someA_sound : return_sound optionA option.
 Proof.
-  unfold bindM; simpl.
-  repeat constructor. intros.
-  destruct m, m'; eauto with soundness.
-Qed.
-Hint Resolve bind_option_sound : soundness.
-
-Lemma someA_sound {A A' : Type} `{GA : Galois A A'} : ∀ (a : A) (a' : A'),
-  γ a a' → 
-  γ (SomeA a) (Some a').
-Proof.
-  eauto with soundness.
+  unfold return_sound; eauto with soundness.
 Qed.
 
-Lemma bind_optionA_sound (A A' B B' : Type) `{Galois A A', Galois B B'} :
-  ∀ (m : optionA A) (m' : option A') 
-    (f : A → optionA B) (f' : A' → option B'),
-  γ m m' → γ f f' →
-  γ (bind_optionA m f) (bind_option m' f').
+Instance bind_optionA_sound : bind_sound optionA option.
 Proof.
-  intros m m' f f' Hm Hf. destruct m, m'; eauto with soundness.
-  - inversion Hm; subst; clear Hm. gamma_destruct. apply H1 in H3.
-    cbv. destruct (f a), (f' a0); simpl; try constructor;  eauto with
-      soundness.
-  - inversion Hm; subst; clear Hm. gamma_destruct. cbv. destruct (f a);
-    constructor.
+  unfold bind_sound; intros. unfold bindM; simpl. destruct m, m'; eauto with
+    soundness.
+  - simpl. gamma_destruct. apply H1 in H3. destruct (f a), (f' a0); eauto with
+    soundness.
+  - simpl. destruct (f a); eauto with soundness.
 Qed.
 
-Lemma bind_state_sound {S S'} `{Galois S S'} : ∀ (A A' B B' : Type)
-  `{Galois A A', Galois B B'},
-  γ
-    (bind_state (S:=S) (A:=A) (B:=B))
-    bind_state.
-Proof. 
-  unfold bind_state. constructor; intros st st' Hst.
-  constructor; intros f f' Hf. constructor; intros s s' Hs.
-  inversion Hst as [?? Hgamma_st]; subst; clear Hst.
-  apply Hgamma_st in Hs. destruct (st' s'), (st s).
-  inversion Hs as [?? Ha Hs']; subst; clear Hs; simpl in *.
-  repeat apply gamma_fun_apply; assumption.
+Instance return_state_sound {S S' : Type} {GS : Galois S S'} : 
+  return_sound (State S) (State S').
+Proof.
+  unfold return_sound; unfold returnM; simpl; intros.
+  constructor. eauto with soundness.
 Qed.
-Hint Resolve bind_state_sound : soundness.
+
+Instance bind_state_sound {S S' : Type} {GS : Galois S S'} :
+  bind_sound (State S) (State S').
+Proof.
+  unfold bind_sound, bindM; simpl; intros.
+  constructor; intros. unfold bind_state. destruct H.
+  apply H in H1. destruct (f0 a), (g a'). eauto with soundness.
+Qed.
 
 Section stateT.
-  Context {M M' : Type → Type} `{Monad M, Monad M'}.
+  Context {M M' : Type → Type} {MM : Monad M} {MM' : Monad M'}.
   Context {GM : ∀ A A', Galois A A' → Galois (M A) (M' A')}.
-  Context {S S' : Type} `{Galois S S'}.
+  Context {S S' : Type} {GS : Galois S S'}.
   Context {RS : return_sound M M'}.
   Context {BS : bind_sound M M'}.
 
-  Lemma return_stateT_sound {A A'} `{Galois A A'} : 
-    γ (return_stateT (S:=S) (M:=M) (A:=A)) 
-      (return_stateT (S:=S') (M:=M') (A:=A')).
+  Global Instance return_stateT_sound : 
+    return_sound (StateT S M) (StateT S' M').
   Proof.
-    unfold return_stateT. constructor. intros a a' Ha. constructor.
-    intros s s' Hs. eauto with soundness.
+    unfold return_sound, returnM; simpl. unfold return_stateT; intros. 
+    eauto with soundness.
   Qed.
 
-  Lemma bind_stateT_sound {A A' B B'} `{Galois A A', Galois B B'} : 
-    ∀ (m : StateT S M A) (m' : StateT S' M' A')
-      (f : A → StateT S M B) (f' : A' → StateT S' M' B'),
-    γ m m' → γ f f' → 
-    γ (bind_stateT m f) (bind_stateT m' f').
+  Global Instance bind_stateT_sound : bind_sound (StateT S M) (StateT S' M').
   Proof.
-    intros. unfold bind_stateT. repeat constructor; intros s s' Hs. 
-    apply bindM_sound.
-    apply gamma_fun_apply; assumption. constructor. intros p p' Hp.
-    destruct p, p'. eauto with soundness.
+    unfold bind_sound, bindM; simpl; unfold bind_stateT; intros.
+    constructor; intros. apply bindM_sound. eauto with soundness.
+    constructor. intros p q Hpq. destruct p, q. eauto with soundness.
   Qed.
 End stateT.
 
 Section optionT.
-  Context {M M' : Type → Type}.
-  Context `{RS : return_sound M M'}.
+  Context {M M' : Type → Type} {MM : Monad M} {MM' : Monad M'}.
+  Context {GM : ∀ A A', Galois A A' → Galois (M A) (M' A')}.
+  Context {RS : return_sound M M'}.
   Context {BS : bind_sound M M'}.
 
-  Lemma someT_sound {A A'} `{Galois A A'} : ∀ a a',
-    γ a a' →
-    γ (returnM (M:=M) (Some a)) (returnM (M:=M') (Some a')).
-  Proof. 
-    intros. eapply gamma_fun_apply; eauto with soundness. 
+  Global Instance someT_sound : return_sound (optionT M) (optionT M').
+  Proof.
+    unfold return_sound, returnM; simpl. intros. eauto with soundness.
   Qed.
 
-  Lemma bind_optionT_sound {A A' B B'} `{Galois A A', Galois B B'} : 
-    ∀ (m : optionT M A) (m' : optionT M' A')
-      (f : A → optionT M B) (f' : A' → optionT M' B'),
-    γ m m' → γ f f' → 
-    γ (bind_optionT m f) (bind_optionT m' f').
-  Proof. 
-    intros. eapply BS. assumption. constructor; intros a a' Ha.
-    gamma_destruct; eauto with soundness. admit.
+  Global Instance bind_optionT_sound : bind_sound (optionT M) (optionT M').
+  Proof.
+    unfold bind_sound, bindM; simpl; intros. 
+    unfold bind_optionT. eapply BS. assumption. constructor.
+    intros. destr; eauto with soundness. 
+    admit.
   Admitted.
 End optionT.
 
 Section optionAT.
-  Context {M M' : Type → Type}.
-  Context `{RS : return_sound M M'} {BS : bind_sound M M'}.
+  Context {M M' : Type → Type} {MM : Monad M} {MM' : Monad M'}.
+  Context {GM : ∀ A A', Galois A A' → Galois (M A) (M' A')}.
+  Context {RS : return_sound M M'}. 
+  Context {BS : bind_sound M M'}.
 
-  Lemma someAT_sound {A A'} `{Galois A A'} : ∀ a a',
-    γ a a' →
-    γ (returnM (SomeA a)) (returnM (Some a')).
-  Proof. eauto with soundness. Qed.
-
-  Lemma bind_optionAT_sound {A A' B B'} `{Galois A A', Galois B B'} : 
-    ∀ (m : optionAT M A) (m' : optionT M' A') 
-      (f : A → optionAT M B) (f' : A' → optionT M' B'),
-    γ m m' → γ f f' →
-    γ (bind_optionAT m f) (bind_optionT m' f').
+  Global Instance someAT_sound : return_sound (optionAT M) (optionT M').
   Proof.
+    unfold return_sound, returnM; simpl.
+    eauto with soundness.
+  Qed.
+
+  Global Instance bind_optionAT : bind_sound (optionAT M) (optionT M').
+  Proof.
+    unfold bind_sound. unfold bindM; simpl.
     intros. unfold bind_optionAT, bind_optionT, optionAT, optionT.
+    unfold bind_sound.
     apply bindM_sound; try assumption.
     constructor; intros a a' Ha.
     inversion Ha; subst; eauto with soundness.
@@ -178,15 +155,14 @@ Section optionAT.
     unfold lift_optionAT, lift_optionT, optionAT, optionT.
     repeat constructor. intros. apply bindM_sound; eauto with soundness.
   Qed.
-
 End optionAT.
 
 (* Soundness of interpreters *)
 
 Definition avalue := ((parity+⊤)+(abstr_bool+⊤))%type.
-Definition ConcreteState := optionT (StateT (store cvalue) (optionT Identity)).
+Definition ConcreteState := optionT (StateT (store cvalue) option).
 
-Definition AbstractState := optionAT (StateT (store (avalue+⊤)) (optionT Identity)).
+Definition AbstractState := optionAT (StateT (store (avalue+⊤)) option).
 
 Theorem eval_expr_sound : forall a,
   γ 
@@ -199,7 +175,10 @@ Proof.
   - auto with soundness.
   - auto with soundness. 
   - auto with soundness.
-  - apply gamma_fun_apply. 2: assumption. admit.
+  - Set Printing Implicit. About γ.
+
+    apply gamma_fun_apply. 2: assumption.
+    admit.
   - admit.
 Admitted.
 Hint Resolve eval_expr_sound : soundness.
